explicit randomness for PKE, remove encryption oracle

uc-dsl/examples/megan/pke_ind_cpa.ec
@@ -11,112 +11,55 @@ type skey.
 type plaintext.
 type ciphertext.
 
+(* randomness *)
+type rand.
+op drand : rand distr.
+axiom dexp_uni : is_uniform drand.
+axiom drand_ll  : is_lossless drand.
+
 op ciph_def : ciphertext.  (* default ciphertext *)
 
-(* Encryption oracle limit before game's encryption.
-   This says limit_pre has type int and the axiom ge0_limit_pre says
-   limit_pre is non-negative *)
-op limit_pre : {int | 0 <= limit_pre} as ge0_limit_pre.
-
-(* Encryption oracle limit after game's encryption. *)
-op limit_post : {int | 0 <= limit_post} as ge0_limit_post.
-
 module type ENC = {
-  proc key_gen(): pkey * skey
-  proc enc(k:pkey, p:plaintext): ciphertext
-  proc dec(k:skey, c:ciphertext): plaintext
+  proc keygen() : pkey * skey
+  proc enc(pk:pkey, m:plaintext, r:rand)  : ciphertext
+  proc dec(sk:skey, c:ciphertext) : plaintext
 }.
 
 (* For checking correctness of encryption scheme *)
 module Correctness (Enc : ENC) = {
   proc main(x : plaintext) : bool = {
-    var pk : pkey; var sk : skey; var c : ciphertext; var y : plaintext;
-    (pk, sk) <@ Enc.key_gen();
-    c <@ Enc.enc(pk, x);
+    var pk : pkey; var sk : skey; var c : ciphertext; var y : plaintext; var r : rand;
+    (pk, sk) <@ Enc.keygen();
+    c <@ Enc.enc(pk, x, r);
     y <@ Enc.dec(sk, c);
     return x = y;
   }
 }.
 
-(* module type of encryption oracles *)
-module type EO = {
-  (* initialization *)
-  proc * init() : unit
-
-  (* encryption of text by adversary before game's encryption *)
-  proc enc_pre(x : plaintext) : ciphertext
-
-  (* one-time encryption of text by game *)
-  proc genc(x : plaintext) : ciphertext
-
-  (* encryption of text by adversary after game's encryption *)
-  proc enc_post(x : plaintext) : ciphertext
-}.
-
-(* standard encryption oracle, constructed from an encryption
-   scheme *)
-module EncO (Enc : ENC) : EO = {
-  var pk : pkey
-  var sk : skey
-  var ctr_pre : int
-  var ctr_post : int
-
-  proc init() : unit = {
-    (pk, sk) <@ Enc.key_gen();
-    ctr_pre <- 0; ctr_post <- 0;
-  }
-
-  proc enc_pre(x : plaintext) : ciphertext = {
-    var c : ciphertext;
-    if (ctr_pre < limit_pre) {
-      ctr_pre <- ctr_pre + 1;
-      c <@ Enc.enc(pk, x);
-    }
-    else {
-      c <- ciph_def;  (* default result *)
-    }  
-    return c;
-  }
-
-  proc genc(x : plaintext) : ciphertext = {
-    var c : ciphertext;
-    c <@ Enc.enc(pk, x);
-    return c;
-  }
-
-  proc enc_post(x : plaintext) : ciphertext = {
-    var c : ciphertext;
-    if (ctr_post < limit_post) {
-      ctr_post <- ctr_post + 1;
-      c <@ Enc.enc(pk, x);
-    }
-    else {
-      c <- ciph_def;  (* default result *)
-    }  
-    return c;
-  }
-}.
-
-module type ADV_INDCPA (EncO : EO) = {
+module type ADV_INDCPA = {
   (* choose a pair of plaintexts *)
-  proc choose(): plaintext * plaintext {EncO.enc_pre}
+  proc choose(): plaintext * plaintext 
 
   (* guess which plaintext was encrypted *)
-  proc guess(c:ciphertext): bool {EncO.enc_post}
+  proc guess(c:ciphertext): bool
 }.
 
 (* IND-CPA Security Game, parametrized by an encryption scheme Enc and ind-cpa adversary *)
 module INDCPA (Enc : ENC, Adv : ADV_INDCPA) = {
-  module EO = EncO(Enc)        (* make EO from Enc *)
-  module A = Adv(EO)           (* connect Adv to EO *)
-
   proc main() : bool = {
-    var b, b' : bool; var x1, x2 : plaintext; var c : ciphertext;
-    EO.init();                 (* initialize EO *)
-    (x1, x2) <@ A.choose();    (* let A choose plaintexts x1/x2 *)
+    var b, b' : bool; 
+    var x1, x2 : plaintext; 
+    var c : ciphertext; 
+    var r : rand; 
+    var pk : pkey;
+    var sk : skey;
+
+    (pk, sk) <@ Enc.keygen();  (* generate keys for PKE *)
+    r <$ drand;                (* select randomness used in PKE *)
+    (x1, x2) <@ Adv.choose();  (* A chooses plaintexts x1/x2 *)
     b <$ {0,1};                (* choose boolean b *)
-    c <@ EO.genc(b ? x1 : x2); (* encrypt x1 if b = true, x2 if b = false *)
-    b' <@ A.guess(c);          (* give ciphertext to A, which returns guess *)
+    c <@ Enc.enc(pk, b ? x1 : x2, r); (* encrypt x1 if b = true, x2 if b = false *)
+    b' <@ Adv.guess(c);        (* give ciphertext to A, which returns guess *)
     return b = b';             (* see if A guessed correctly, winning game *)
   }
 }.
